clightplus_examples/vector/vector1.v
@@ -19,45 +19,90 @@ Section PROP.
   Context `{@GRA.inG blocksizeRA Σ}.
   Context `{@GRA.inG blockaddressRA Σ}.
 
-  (* Variable (item : Type) (item_size : item -> nat). *)
+  Inductive cell : Type :=
+  | owned (mvs : list memval) (q : Qp)
+  | lent (size : nat)
+  .
 
-  Definition VECTOR_INIT_CAPACITY := 4.
-  Definition vector_struct_size := (size_chunk Mptr + 3 * (size_chunk Mint64))%Z.
-
-  Definition is_vector_handler q (handler items size capacity total: val) : iProp :=
-    (∃ m tag offset,
-      handler (↦_m,q) (encode_val Mptr items ++ flat_map (encode_val Mint64) [size; capacity; total])
-      ** handler (⊨_m,tag,q) offset
-      ** ⌜(vector_struct_size | Ptrofs.unsigned offset)%Z⌝)%I.
-
-  (* block m is allocated with qb fractional resource which is distributed over the list *)
-  Definition valid_entry m ptr ofs vl qv size : iProp :=
-    ptr (↦_m,qv) vl
-    ** ⌜bytes_not_pure vl = false⌝
-    ** ⌜(Z.of_nat size | Ptrofs.unsigned ofs)%Z⌝
-    ** ⌜Datatypes.length vl = size⌝.
-
-  Fixpoint list_points_to ptr m ofs memlist size : iProp :=
-    match memlist with
-    | [] => True%I
-    | (ml, qv) :: tl =>
-        valid_entry m ptr ofs ml qv size
-        ** list_points_to
-          (Val.addl ptr (Vptrofs (Ptrofs.repr size))) m (Ptrofs.add ofs (Ptrofs.repr size)) tl size
+  Definition cell_size (c : cell) : nat :=
+    match c with
+    | owned mvs q => Datatypes.length mvs
+    | lent size => size
     end.
 
-  (* total <= capacity <= size * capacity <= Ptrofs.max_unsigned *)
-  Definition is_vector vm qh qb handler (size capacity total : nat) (memlist : list ((list memval) * Qp)) : iProp :=
-    (∃ items unused,
-      ⌜capacity <= size * capacity <= Z.to_nat Ptrofs.max_unsigned
-      /\ total <= capacity
-      /\ Datatypes.length memlist = total
-      /\ (total + (Datatypes.length unused))%nat = capacity
-      /\ Forall (fun a => a.2 = 1%Qp) unused⌝
-      ** is_vector_handler qh handler items
-          (Vlong (Int64.repr size)) (Vlong (Int64.repr capacity)) (Vlong (Int64.repr total))
-      ** list_points_to items vm Ptrofs.zero (memlist ++ unused) size
-      ** items (⊨_vm,Dynamic,qb) Ptrofs.zero)%I.
+  Definition cell_points_to (ptr : val) (m : metadata) (c : cell) : iProp :=
+    match c with
+    | owned mvs q => ptr (↦_m,q) mvs
+    | lent size => True%I
+    end.
+
+  Fixpoint list_points_to ptr m (cs : list cell) : iProp :=
+    match cs with
+    | [] => True%I
+    | c :: cs' => cell_points_to ptr m c ** list_points_to (Val.addl ptr (Vptrofs (Ptrofs.repr (cell_size c)))) m cs'
+    end.
+
+  Definition is_vector_handler (v : val) (data : val) (esize capacity length: nat) mᵥ tgᵥ pᵥ qᵥ : iProp :=
+    ( ∃ ofsᵥ,
+      ⌜ (8 | Ptrofs.unsigned ofsᵥ)%Z ⌝
+      ∗ v (↦_mᵥ,pᵥ) (encode_val Mptr data
+                       ++ encode_val Mint64 (Vlong (Int64.repr esize))
+                       ++ encode_val Mint64 (Vlong (Int64.repr capacity))
+                       ++ encode_val Mint64 (Vlong (Int64.repr length)))
+      ∗ v (⊨_mᵥ,tgᵥ,qᵥ) ofsᵥ
+    )%I.
+
+  Definition is_vector_fixed (v : val) (data : val) (esize capacity length : nat) (cells : list cell) mᵥ tgᵥ pᵥ qᵥ m_data q_data : iProp :=
+    ( ⌜ esize > 0
+      /\ capacity > 0
+      /\ esize * capacity <= Z.to_nat Ptrofs.max_unsigned
+      /\ length <= capacity
+      /\ Datatypes.length cells = length
+      /\ Forall (fun c => cell_size c = esize) cells
+      ⌝
+      ∗ is_vector_handler v data esize capacity length mᵥ tgᵥ pᵥ qᵥ
+      ∗ list_points_to data m_data cells
+      ∗ data (⊨_m_data,Dynamic,q_data) Ptrofs.zero
+    )%I.
+
+  Definition is_vector (v : val) (esize capacity length : nat) (cells : list cell) mᵥ tgᵥ qᵥ : iProp :=
+    ( ∃ (data : val) (m_data : metadata) (unused_length : nat) (unused : list memval),
+      ⌜ esize > 0
+      /\ capacity > 0
+      /\ esize * capacity <= Z.to_nat Ptrofs.max_unsigned
+      /\ (length + unused_length)%nat = capacity
+      /\ Datatypes.length cells = length
+      /\ Datatypes.length unused = (esize * unused_length)%nat
+      /\ Forall (fun c => cell_size c = esize) cells
+      /\ Forall (fun c => exists mvs, c = owned mvs 1) cells
+      ⌝
+      ∗ is_vector_handler v data esize capacity length mᵥ tgᵥ 1 qᵥ
+      ∗ list_points_to data m_data cells
+      ∗ data (⊨_m_data,Dynamic,1) Ptrofs.zero
+      ∗ (Val.addl data (Vptrofs (Ptrofs.repr (esize * length)))) (↦_m_data,1) unused
+    )%I.
+
+  Lemma is_vector_fix
+    v esize capacity length cells mᵥ tgᵥ qᵥ
+    : bi_entails
+        (is_vector v esize capacity length cells mᵥ tgᵥ qᵥ)
+        (∃ data m_data,
+            ⌜ Forall (fun c => exists mvs, c = owned mvs 1) cells ⌝
+            ∗ is_vector_fixed v data esize capacity length cells mᵥ tgᵥ 1 qᵥ m_data 1
+            ∗ (∀ qᵥ' cells',
+                ⌜ Forall (fun c => exists mvs, c = owned mvs 1) cells' ⌝
+                -∗ is_vector_fixed v data esize capacity length cells' mᵥ tgᵥ 1 qᵥ' m_data 1
+                -∗ is_vector v esize capacity length cells' mᵥ tgᵥ qᵥ' )).
+  Proof.
+    iIntros "V".
+    iDestruct "V" as (data m_data unused_length unused) "[% [V1 [V2 [V3 V4]]]]". des.
+    iExists data, m_data. iSplit; ss. iSplitL "V1 V2 V3".
+    - iFrame. iPureIntro. splits; ss; lia.
+    - iIntros (qᵥ' cells') "% V".
+      iDestruct "V" as "[% [V1 [V2 V3]]]". des.
+      iExists data, m_data, (capacity - length), unused.
+      iFrame. iPureIntro. splits; ss; lia.
+  Qed.
 
 End PROP.
 
@@ -68,144 +113,211 @@ Section SPEC.
   Context `{@GRA.inG blocksizeRA Σ}.
   Context `{@GRA.inG blockaddressRA Σ}.
 
+  (* TODO : Fix specs *)
   Definition vector_init_spec : fspec :=
-    mk_simple
-      (fun '(vec_ptr, size) => (
-        (ord_pure 1%nat),
-        (fun varg =>
-          ∃ items usize capacity total,
-          ⌜varg = [vec_ptr; Vlong (Int64.repr (size : nat))]↑
-          /\ (0 < size * VECTOR_INIT_CAPACITY <= Z.to_nat Ptrofs.max_unsigned)%Z⌝
-          ** is_vector_handler 1 vec_ptr items usize capacity total)%I,
-        (fun vret =>
-          ⌜vret = Vundef↑⌝
-          ** ∃ m, is_vector m 1 1 vec_ptr size VECTOR_INIT_CAPACITY 0 [])
-      )).
+    @mk_simple
+      _
+      (val * nat * nat * metadata * tag * Qp * list memval * ptrofs)
+      (fun '(v, esize, capacity, mᵥ, tgᵥ, qᵥ, mvsᵥ, ofsᵥ) =>
+         ( ord_pure 1%nat
+         , fun varg =>
+             ⌜ varg = [v; Vlong (Int64.repr esize); Vlong (Int64.repr capacity)]↑
+             /\ esize > 0
+             /\ capacity > 0
+             /\ esize * capacity <= Z.to_nat Ptrofs.max_unsigned
+             /\ Datatypes.length mvsᵥ = 24
+             ⌝
+             ∗ v (↦_mᵥ,1) mvsᵥ
+             ∗ v (⊨_mᵥ,tgᵥ,qᵥ) ofsᵥ
+         , fun vret =>
+             ⌜vret = Vundef↑⌝
+             ∗ is_vector v esize capacity 0 [] mᵥ tgᵥ qᵥ
+         )%I
+      ).
 
-  Definition vector_total_spec : fspec :=
-    mk_simple
-      (fun '(vec_ptr, vec_m, size, capacity, total, memlist, q, qb) => (
-        (ord_pure 1%nat),
-        (fun varg =>
-          ⌜varg = [vec_ptr]↑⌝
-          ** is_vector vec_m q qb vec_ptr size capacity total memlist)%I,
-        (fun vret =>
-          ⌜vret = (Vlong (Int64.repr total))↑⌝
-          ** is_vector vec_m q qb vec_ptr size capacity total memlist)
-      )).
+  Definition vector_destruct_spec : fspec :=
+    @mk_simple
+      _
+      (val * nat * nat * nat * list cell * metadata * tag * Qp)
+      (fun '(v, esize, capacity, length, cells, mᵥ, tgᵥ, qᵥ) =>
+         ( ord_pure 1%nat
+         , fun varg =>
+             ⌜varg = [v]↑⌝
+             ∗ is_vector v esize capacity length cells mᵥ tgᵥ qᵥ
+         , fun vret =>
+             ∃ mvsᵥ ofsᵥ,
+             ⌜vret = Vundef↑⌝
+             ∗ v (↦_mᵥ,1) mvsᵥ
+             ∗ v (⊨_mᵥ,tgᵥ,qᵥ) ofsᵥ
+         )%I
+      ).
 
-  Definition vector_resize_spec : fspec :=
-    mk_simple
-      (fun '(newcap, size, total, memlist) => (
-        (ord_pure 1%nat),
-        (fun varg =>
-          ∃ vec_ptr vec_m oldcap,
-          ⌜varg = [vec_ptr; (Vlong (Int64.repr (newcap : nat)))]↑
-          /\ 0 < newcap * size < (Z.to_nat Ptrofs.max_unsigned)
-          /\ total < newcap⌝
-          ** is_vector vec_m 1 1 vec_ptr size oldcap total memlist)%I,
-        (fun vret =>
-          ∃ vec_m' vec_ptr',
-          ⌜vret = Vundef↑⌝
-          ** is_vector vec_m' 1 1 vec_ptr' size newcap total memlist))
-      )%I.
+  Definition vector_esize_spec : fspec :=
+    @mk_simple
+      _
+      (val * val * nat * nat * nat * list cell * metadata * tag * Qp * Qp * metadata * Qp)
+      (fun '(v, data, esize, capacity, length, cells, mᵥ, tgᵥ, pᵥ, qᵥ, m_data, q_data) =>
+         ( ord_pure 1%nat
+         , fun varg =>
+             ⌜varg = [v]↑⌝
+             ∗ is_vector_fixed v data esize capacity length cells mᵥ tgᵥ pᵥ qᵥ m_data q_data
+         , fun vret =>
+             ⌜vret = (Vlong (Int64.repr esize))↑⌝
+             ∗ is_vector_fixed v data esize capacity length cells mᵥ tgᵥ pᵥ qᵥ m_data q_data
+         )%I
+      ).
 
-  (* TODO: to be revised *)
-  Definition vector_add_spec : fspec :=
-    mk_simple
-      (fun '(vec_ptr, item_ptr, vec_m, vec_m', item, m, size, capacity, total, memlist, qitem, qbitem, tagitem, ofs) => (
-        (ord_pure 1%nat),
-        (fun varg =>
-          ⌜varg = [vec_ptr; item_ptr]↑
-          /\ Datatypes.length item = size⌝
-          ** is_vector vec_m 1 1 vec_ptr size capacity total memlist
-          ** item_ptr (↦_m,qitem) item
-          ** item_ptr (⊨_m,tagitem,qbitem) ofs),
-        (fun vret =>
-          ⌜vret = Vundef↑⌝
-          ** (if total <? capacity
-              then is_vector vec_m 1 1 vec_ptr size capacity (total + 1) (memlist ++ [(item, 1%Qp)])
-              else if capacity <? Z.to_nat Ptrofs.half_modulus
-                then is_vector vec_m' 1 1 vec_ptr size (2 * capacity) (total + 1) (memlist ++ [(item, 1%Qp)])
-                else True%I)
-          ** item_ptr (↦_m,qitem) item
-          ** item_ptr (⊨_m,tagitem,qbitem) ofs)
-      )).
+  Definition vector_capacity_spec : fspec :=
+    @mk_simple
+      _
+      (val * val * nat * nat * nat * list cell * metadata * tag * Qp * Qp * metadata * Qp)
+      (fun '(v, data, esize, capacity, length, cells, mᵥ, tgᵥ, pᵥ, qᵥ, m_data, q_data) =>
+         ( ord_pure 1%nat
+         , fun varg =>
+             ⌜varg = [v]↑⌝
+             ∗ is_vector_fixed v data esize capacity length cells mᵥ tgᵥ pᵥ qᵥ m_data q_data
+         , fun vret =>
+             ⌜vret = (Vlong (Int64.repr capacity))↑⌝
+             ∗ is_vector_fixed v data esize capacity length cells mᵥ tgᵥ pᵥ qᵥ m_data q_data
+         )%I
+      ).
 
-  Definition vector_set_spec : fspec :=
-    mk_simple
-      (fun '(vec_ptr, idx, item_ptr, vec_m, item, m, size, capacity, total, l1, old, l2, qb, qh, qitem, qbitem, tagitem, ofs) => (
-        (ord_pure 1%nat),
-        (fun varg =>
-          ⌜varg = [vec_ptr; (Vlong (Int64.repr (idx : nat))); item_ptr]↑
-          /\ Datatypes.length item = size
-          /\ Datatypes.length l1 = idx⌝
-          ** is_vector vec_m qh qb vec_ptr size capacity total (l1 ++ (old, 1%Qp) :: l2)
-          ** item_ptr (↦_m,qitem) item
-          ** item_ptr (⊨_m,tagitem,qbitem) ofs),
-        (fun vret =>
-          ⌜vret = Vundef↑⌝
-          ** is_vector vec_m qh qb vec_ptr size capacity total (l1 ++ (item, 1%Qp) :: l2)
-          ** item_ptr (↦_m,qitem) item
-          ** item_ptr (⊨_m,tagitem,qbitem) ofs)
-      )).
+  Definition vector_length_spec : fspec :=
+    @mk_simple
+      _
+      (val * val * nat * nat * nat * list cell * metadata * tag * Qp * Qp * metadata * Qp)
+      (fun '(v, data, esize, capacity, length, cells, mᵥ, tgᵥ, pᵥ, qᵥ, m_data, q_data) =>
+         ( ord_pure 1%nat
+         , fun varg =>
+             ⌜varg = [v]↑⌝
+             ∗ is_vector_fixed v data esize capacity length cells mᵥ tgᵥ pᵥ qᵥ m_data q_data
+         , fun vret =>
+             ⌜vret = (Vlong (Int64.repr length))↑⌝
+             ∗ is_vector_fixed v data esize capacity length cells mᵥ tgᵥ pᵥ qᵥ m_data q_data
+         )%I
+      ).
+
+  Definition vector_reserve_spec : fspec :=
+    @mk_simple
+      _
+      (val * nat * nat * nat * list cell * metadata * tag * Qp * nat)
+      (fun '(v, esize, capacity, length, cells, mᵥ, tgᵥ, qᵥ, min_capacity) =>
+         ( ord_pure 1%nat
+         , fun varg =>
+             ⌜varg = [v; Vlong (Int64.repr min_capacity)]↑
+             /\ min_capacity > 0
+             /\ esize * min_capacity < Z.to_nat Ptrofs.max_unsigned
+             ⌝
+             ∗ is_vector v esize capacity length cells mᵥ tgᵥ qᵥ
+         , fun vret =>
+             ⌜vret = Vundef↑⌝
+             ∗ is_vector v esize (max capacity min_capacity) length cells mᵥ tgᵥ qᵥ
+         )%I
+      ).
+
+  Definition vector_push_spec : fspec :=
+    @mk_simple
+      _
+      (val * nat * nat * nat * list cell * metadata * tag * Qp *
+         val * list memval * ptrofs * metadata * tag * Qp * Qp)
+      (fun '(v, esize, capacity, length, cells, mᵥ, tgᵥ, qᵥ,
+           src, mvs_src, ofs_src, m_src, tg_src, p_src, q_src) =>
+         ( ord_pure 1%nat
+         , fun varg =>
+             ⌜varg = [v; src]↑
+             /\ Datatypes.length mvs_src = esize
+             ⌝
+             ∗ is_vector v esize capacity length cells mᵥ tgᵥ qᵥ
+             ∗ src (↦_m_src,p_src) mvs_src
+             ∗ src (⊨_m_src,tg_src,q_src) ofs_src
+         , fun vret =>
+             ∃ capacity',
+             ⌜vret = Vundef↑⌝
+             ∗ is_vector v esize capacity' length (cells ++ [owned mvs_src 1]) mᵥ tgᵥ qᵥ
+             ∗ src (↦_m_src,p_src) mvs_src
+             ∗ src (⊨_m_src,tg_src,q_src) ofs_src
+         )%I
+      ).
 
   Definition vector_get_spec : fspec :=
-    mk_simple
-      (fun '(vec_ptr, idx, vec_m, qh, item_ptr, item, qi, size, capacity, total, qb, l1, l2) => (
-        (ord_pure 1%nat),
-        (fun varg =>
-          ⌜varg = [vec_ptr; (Vlong (Int64.repr (idx : nat)))]↑
-          /\ Datatypes.length l1 = idx⌝
-          ** is_vector vec_m qh qb vec_ptr size capacity total (l1 ++ (item, qi) :: l2)),
-        (fun vret =>
-          ⌜vret = item_ptr↑⌝
-          ** is_vector vec_m qh (qb/2) vec_ptr size capacity total (l1 ++ (item, qi/2) :: l2)%Qp
-          ** item_ptr (↦_vec_m,qi/2) item
-          ** item_ptr (⊨_vec_m,Dynamic,qb/2) (Ptrofs.add Ptrofs.zero (Ptrofs.repr (idx * size))))
-      )).
+    @mk_simple
+      _
+      (val * val * nat * nat * nat * list cell * metadata * tag * Qp * Qp * metadata * Qp *
+         nat * list memval * Qp * val * list memval * ptrofs * metadata * tag * Qp)
+      (fun '(v, data, esize, capacity, length, cells, mᵥ, tgᵥ, pᵥ, qᵥ, m_data, q_data,
+           index, mvs_index, p_index, dst, mvs_dst, ofs_dst, m_dst, tg_dst, q_dst) =>
+         ( ord_pure 1%nat
+         , fun varg =>
+             ⌜ varg = [v; Vlong (Int64.repr (index : nat)); dst]↑
+             /\ cells !! index = Some (owned mvs_index p_index)
+             /\ Datatypes.length mvs_dst = esize
+             ⌝
+             ∗ is_vector_fixed v data esize capacity length cells mᵥ tgᵥ pᵥ qᵥ m_data q_data
+             ∗ dst (↦_m_dst,1) mvs_dst
+             ∗ dst (⊨_m_dst,tg_dst,q_dst) ofs_dst
+         , fun vret =>
+             ⌜vret = Vundef↑⌝
+             ∗ is_vector_fixed v data esize capacity length cells mᵥ tgᵥ pᵥ qᵥ m_data q_data
+             ∗ dst (↦_m_dst,1) mvs_index
+             ∗ dst (⊨_m_dst,tg_dst,q_dst) ofs_dst
+         )%I
+      ).
 
-  (* TODO: to be revised *)
-  Definition vector_delete_spec : fspec :=
-    (mk_simple
-      (fun '(vec_ptr, idx, vec_m, vec_m', size, capacity, total, l1, item, l2) => (
-        (ord_pure 1%nat),
-        (fun varg =>
-          ⌜varg = [vec_ptr; (Vlong (Int64.repr (idx : nat)))]↑
-          /\ Datatypes.length l1 = idx
-          /\ Forall (fun a => a.2 = 1%Qp) (l1 ++ l2)⌝
-          ** is_vector vec_m 1 1 vec_ptr size capacity (S total) (l1 ++ (item, 1%Qp) :: l2)),
-        (fun vret => ⌜vret = Vundef↑⌝
-          ** (if (0 <? total) && (total =? (capacity / 4))%nat
-              then is_vector vec_m' 1 1 vec_ptr size (capacity / 2) total (l1 ++ l2)
-              else is_vector vec_m 1 1 vec_ptr size capacity total (l1 ++ l2)))
-    )))%I.
+  Definition vector_set_spec : fspec :=
+    @mk_simple
+      _
+      (val * val * nat * nat * nat * list cell * metadata * tag * Qp * Qp * metadata * Qp *
+         nat * list memval * val * list memval * ptrofs * metadata * tag * Qp * Qp)
+      (fun '(v, data, esize, capacity, length, cells, mᵥ, tgᵥ, pᵥ, qᵥ, m_data, q_data,
+           index, mvs_index, src, mvs_src, ofs_src, m_src, tg_src, p_src, q_src) =>
+         ( ord_pure 1%nat
+         , fun varg =>
+             ⌜ varg = [v; Vlong (Int64.repr (index : nat)); src]↑
+             /\ cells !! index = Some (owned mvs_index 1)
+             /\ Datatypes.length mvs_src = esize
+             ⌝
+             ∗ is_vector_fixed v data esize capacity length cells mᵥ tgᵥ pᵥ qᵥ m_data q_data
+             ∗ src (↦_m_src,p_src) mvs_src
+             ∗ src (⊨_m_src,tg_src,q_src) ofs_src
+         , fun vret =>
+             ⌜vret = Vundef↑⌝
+             ∗ is_vector_fixed v data esize capacity length (<[index := owned mvs_src 1]> cells) mᵥ tgᵥ pᵥ qᵥ m_data q_data
+             ∗ src (↦_m_src,p_src) mvs_src
+             ∗ src (⊨_m_src,tg_src,q_src) ofs_src
+         )%I
+      ).
 
-  Definition vector_free_spec : fspec :=
-    (mk_simple
-      (fun '(vec_ptr, vec_m, size, capacity, total, memlist, items) => (
-        (ord_pure 1%nat),
-        (fun varg => ⌜varg = [vec_ptr]↑⌝
-          ** is_vector vec_m 1 1 vec_ptr size capacity total memlist),
-        (fun vret => ⌜vret = Vundef↑⌝
-          ** is_vector_handler 1 vec_ptr items
-            (Vlong (Int64.repr size)) (Vlong (Int64.repr capacity)) (Vlong (Int64.repr total)))
-    )))%I.
-    
+  Definition vector_remove_spec : fspec :=
+    @mk_simple
+      _
+      (val * nat * nat * nat * list cell * metadata * tag * Qp * nat * list memval)
+      (fun '(v, esize, capacity, length, cells, mᵥ, tgᵥ, qᵥ, index, mvs_index) =>
+         ( ord_pure 1%nat
+         , fun varg =>
+             ⌜varg = [v; (Vlong (Int64.repr (index : nat)))]↑
+             /\ cells !! index = Some (owned mvs_index 1)
+             ⌝
+             ∗ is_vector v esize capacity length cells mᵥ tgᵥ qᵥ
+         , fun vret =>
+             ⌜vret = Vundef↑⌝
+             ∗ is_vector v esize capacity (length - 1) (delete index cells) mᵥ tgᵥ qᵥ
+         )%I
+      ).
+
   (* sealed *)
-  Definition vectorStb : list (gname * fspec).
-    eapply (Seal.sealing "stb").
-    apply [
-           ("vector_init", vector_init_spec);
-           ("vector_total", vector_total_spec);
-           ("vector_resize", vector_resize_spec);
-           ("vector_add", vector_add_spec);
-           ("vector_set", vector_set_spec);
-           ("vector_get", vector_get_spec);
-           ("vector_delete", vector_delete_spec);
-           ("vector_free", vector_free_spec)
-           ].
-  Defined.
+  Definition vectorStb : list (gname * fspec) :=
+    Seal.sealing "stb" [
+        ("vector_init",    vector_init_spec);
+        ("vector_destruct", vector_destruct_spec);
+        ("vector_esize",    vector_esize_spec);
+        ("vector_capacity", vector_capacity_spec);
+        ("vector_length",   vector_length_spec);
+        ("vector_reserve",  vector_reserve_spec);
+        ("vector_push",     vector_push_spec);
+        ("vector_get",      vector_get_spec);
+        ("vector_set",      vector_set_spec);
+        ("vector_remove",   vector_remove_spec)
+      ].
 
 End SPEC.
 
@@ -218,14 +330,16 @@ Section SMOD.
 
   Definition vectorSbtb: list (gname * fspecbody) :=
     [
-      ("vector_init", mk_pure vector_init_spec);
-      ("vector_total", mk_pure vector_total_spec);
-      ("vector_resize", mk_pure vector_resize_spec);
-      ("vector_add", mk_pure vector_add_spec);
-      ("vector_set", mk_pure vector_set_spec);
-      ("vector_get", mk_pure vector_get_spec);
-      ("vector_delete", mk_pure vector_delete_spec);
-      ("vector_free", mk_pure vector_free_spec)
+      ("vector_init",     mk_pure vector_init_spec);
+      ("vector_destruct", mk_pure vector_destruct_spec);
+      ("vector_esize",    mk_pure vector_esize_spec);
+      ("vector_capacity", mk_pure vector_capacity_spec);
+      ("vector_length",   mk_pure vector_length_spec);
+      ("vector_reserve",  mk_pure vector_reserve_spec);
+      ("vector_push",     mk_pure vector_push_spec);
+      ("vector_get",      mk_pure vector_get_spec);
+      ("vector_set",      mk_pure vector_set_spec);
+      ("vector_remove",   mk_pure vector_remove_spec)
     ].
   
   Definition SvectorSem : SModSem.t := {|
